@prefix rdf:  <http://www.w3.org/1999/02/22-rdf-syntax-ns#> .
@prefix rdfs: <http://www.w3.org/2000/01/rdf-schema#> .
@prefix owl:  <http://www.w3.org/2002/07/owl#> .
@prefix nary: <http://gallows.inf.ed.ac.uk/schema/n-ary#> .

nary:Relation a owl:Class ;
    rdfs:label "(reified) n-ary relation" ;
    rdfs:comment """
The class of resources such as are often used in RDF
to represent non-binary relations. An example is the
org:Membership class, which is used to relate an agent,
an organisation and a role as in,

    nary:m a org:Membership ;
        org:member <http://example.org/people/alice> ;
        org:organisation <http://example.org/org> ;
        org:role <http://example.org/roles/president> .

then we can also say,

    org:Membership a nary:Relation .
""" .

nary:reifiedType a owl:ObjectProperty ;
    rdfs:label "reified type" ;
    rdfs:domain nary:CurriedRelation ;
    rdfs:range nary:Relation ;
    rdfs:comment """
The nary:reifiedType property connects a nary:CurriedRelation to
the reified complete nary:Relation that it expands to when
all arguments are uncurried.
""" .

nary:CurriedRelation a owl:Class ;
    rdfs:label "curried relation" ;
    rdfs:subClassOf
        rdf:Property, [
            a owl:Restriction ; 
            owl:onProperty nary:reifiedType ;
            owl:minCardinality 1
        ], [
            a owl:Restriction ;
            owl:onProperty nary:arg ;
            owl:minCardinality 1
        ] ;
    rdfs:comment """
A nary:CurriedRelation is a type of predicate that contains
extra information to support the creation of an instance of
an nary:Relation. In particular it must have at least one
one statement with nary:reifiedType, and at least one statement
with nary:arg indicating the information that is implicitly
carried along.
""" .

nary:arg a rdf:Property ;
    rdfs:label "argument" ;
    rdfs:domain nary:CurriedRelation ;
    rdfs:range rdf:Resource ;
    rdfs:comment """
nary:arg connects a nary:CurriedRelation to a curried
nary:Argument.
""" .

nary:predicate a owl:ObjectProperty ;
    rdfs:label "predicate" ;
    rdfs:domain nary:Argument ;
    rdfs:range rdf:Property ;
    rdfs:comment """
nary:predicate indicates, for a particular curried nary:Argument,
the predicate that would be present if the curried relation were
expanded to full reified form.
""" .

nary:object a rdf:Property ;
    rdfs:label "object" ;
    rdfs:domain nary:Argument ;
    rdfs:comment """
nary:object indicates, for a particular curried nary:Argument,
the object that would be present if the curried relation were 
expanded to full reified form.
""" .

nary:subjectPredicate a owl:ObjectProperty ;
    rdfs:label "subject" ;
    rdfs:domain nary:BinaryRelation ;
    rdfs:range rdf:Property ;
    rdfs:comment """
nary:subjectPredicate indicates, for a particular nary:BinaryRelation,
which predicate to use for the subject of that relation when
constructing the reified equivalent.
""" .

nary:objectPredicate a owl:ObjectProperty ;
    rdfs:label "object" ;
    rdfs:domain nary:BinaryRelation ;
    rdfs:range rdf:Property ;
    rdfs:comment """
nary:objectPredicate indicates, for a particular nary:BinaryRelation,
which predicate to use for the object of that relation when
constructing the reified equivalent.
""" .

nary:BinaryRelation a owl:Class ;
    rdfs:label "binary relation" ;
    owl:EquivalentClass rdf:Property ;
    rdfs:subClassOf
        nary:CurriedRelation, [
            a owl:Restriction ;
            owl:onProperty nary:subjectPredicate ;
            owl:minCardinality 1 ;
            owl:maxCardinality 1 ;
        ], [
            a owl:Restriction ;
            owl:onProperty nary:objectPredicate ;
            owl:minCardinality 1 ;
            owl:maxCardinality 1 ;
        ] ;
    rdfs:comment """
An nary:BinaryRelation is the only kind of "complete" nary:CurriedRelation
in that it can be used to automatically instantiate the equivalent
nary:Relation. It must have an nary:subjectPredicate and an
nary:objectPredicate.
""" .